<?xml version="1.0"?>
<rdf:RDF xmlns="http://www.parameter_estimation_ontology.org#"
     xml:base="http://www.parameter_estimation_ontology.org"
     xmlns:dc="http://purl.org/dc/elements/1.1/"
     xmlns:obo="http://purl.obolibrary.org/obo/"
     xmlns:owl="http://www.w3.org/2002/07/owl#"
     xmlns:rdf="http://www.w3.org/1999/02/22-rdf-syntax-ns#"
     xmlns:xml="http://www.w3.org/XML/1998/namespace"
     xmlns:xsd="http://www.w3.org/2001/XMLSchema#"
     xmlns:foaf="http://xmlns.com/foaf/0.1/"
     xmlns:rdfs="http://www.w3.org/2000/01/rdf-schema#"
     xmlns:terms="http://purl.org/dc/terms/"
     xmlns:protege="http://protege.stanford.edu/plugins/owl/protege#"
     xmlns:oboInOwl="http://www.geneontology.org/formats/oboInOwl#">
    <owl:Ontology rdf:about="http://www.parameter_estimation_ontology.org">
        <owl:imports rdf:resource="http://purl.obolibrary.org/obo/bfo/2019-08-26/bfo.owl"/>
        <owl:imports rdf:resource="http://purl.obolibrary.org/obo/iao/2020-12-09/iao.owl"/>
    </owl:Ontology>
    


    <!-- 
    ///////////////////////////////////////////////////////////////////////////////////////
    //
    // Object Properties
    //
    ///////////////////////////////////////////////////////////////////////////////////////
     -->

    


    <!-- http://www.parameter_estimation_ontology.org#describes_model_error_scatter_of -->

    <owl:ObjectProperty rdf:about="http://www.parameter_estimation_ontology.org#describes_model_error_scatter_of">
        <owl:inverseOf rdf:resource="http://www.parameter_estimation_ontology.org#model_error_scatter_described_by"/>
        <rdfs:domain rdf:resource="http://purl.obolibrary.org/obo/IAO_0000029"/>
        <rdfs:range rdf:resource="http://www.parameter_estimation_ontology.org#output_sensor"/>
        <obo:IAO_0000115 xml:lang="en">A relation between a numeral and an output sensor where the former describes the scatter (for example the standard deviation) of the difference between the model prediction returned by the output sensor and the corresponding experimental data.</obo:IAO_0000115>
        <obo:IAO_0000117 xml:lang="en">PERSON: Alexander Klawonn</obo:IAO_0000117>
        <rdfs:label xml:lang="en">describes model error scatter of</rdfs:label>
    </owl:ObjectProperty>
    


    <!-- http://www.parameter_estimation_ontology.org#deterministically_models_experiment -->

    <owl:ObjectProperty rdf:about="http://www.parameter_estimation_ontology.org#deterministically_models_experiment">
        <owl:inverseOf rdf:resource="http://www.parameter_estimation_ontology.org#is_deterministically_modeled_by"/>
        <rdfs:domain rdf:resource="http://www.parameter_estimation_ontology.org#forward_model"/>
        <rdfs:range rdf:resource="http://www.parameter_estimation_ontology.org#single_experiment_data_set"/>
        <obo:IAO_0000115 xml:lang="en">A relation between a forward model and a single experiment data set where the former describes some part of the data of the later in deterministic terms (i.e., without considering uncertainty).</obo:IAO_0000115>
        <obo:IAO_0000117 xml:lang="en">PERSON: Alexander Klawonn</obo:IAO_0000117>
        <rdfs:label xml:lang="en">deterministically models experiment</rdfs:label>
    </owl:ObjectProperty>
    


    <!-- http://www.parameter_estimation_ontology.org#has_argument -->

    <owl:ObjectProperty rdf:about="http://www.parameter_estimation_ontology.org#has_argument">
        <rdfs:domain rdf:resource="http://www.parameter_estimation_ontology.org#mathematical_function"/>
        <rdfs:range rdf:resource="http://purl.obolibrary.org/obo/IAO_0000029"/>
        <obo:IAO_0000115 xml:lang="en">A relation between a mathematical function and a numeral where the latter serves as an input to the former.</obo:IAO_0000115>
        <obo:IAO_0000117 xml:lang="en">PERSON: Alexander Klawonn</obo:IAO_0000117>
        <rdfs:label xml:lang="en">has argument</rdfs:label>
    </owl:ObjectProperty>
    


    <!-- http://www.parameter_estimation_ontology.org#has_constant -->

    <owl:ObjectProperty rdf:about="http://www.parameter_estimation_ontology.org#has_constant">
        <rdfs:subPropertyOf rdf:resource="http://purl.obolibrary.org/obo/BFO_0000051"/>
        <rdfs:domain rdf:resource="http://www.parameter_estimation_ontology.org#inverse_problem"/>
        <rdfs:range rdf:resource="http://www.parameter_estimation_ontology.org#constant"/>
        <obo:IAO_0000115 xml:lang="en">A relation between an inverse problem and a constant indicating that the latter is part of the definition of the former.</obo:IAO_0000115>
        <obo:IAO_0000117 xml:lang="en">PERSON: Alexander Klawonn</obo:IAO_0000117>
        <rdfs:label xml:lang="en">has constant</rdfs:label>
    </owl:ObjectProperty>
    


    <!-- http://www.parameter_estimation_ontology.org#has_correlation_length -->

    <owl:ObjectProperty rdf:about="http://www.parameter_estimation_ontology.org#has_correlation_length">
        <rdfs:subPropertyOf rdf:resource="http://www.parameter_estimation_ontology.org#has_argument"/>
        <rdfs:domain rdf:resource="http://www.parameter_estimation_ontology.org#correlation_function"/>
        <rdfs:range rdf:resource="http://purl.obolibrary.org/obo/IAO_0000029"/>
        <obo:IAO_0000115 xml:lang="en">A relation between a correlation function and a numeral that represents a correlation length where the latter serves as an input to the former.</obo:IAO_0000115>
        <obo:IAO_0000117 xml:lang="en">PERSON: Alexander Klawonn</obo:IAO_0000117>
        <rdfs:label xml:lang="en">has correlation length</rdfs:label>
    </owl:ObjectProperty>
    


    <!-- http://www.parameter_estimation_ontology.org#has_covariance_matrix -->

    <owl:ObjectProperty rdf:about="http://www.parameter_estimation_ontology.org#has_covariance_matrix">
        <rdfs:subPropertyOf rdf:resource="http://www.parameter_estimation_ontology.org#has_argument"/>
        <rdfs:domain rdf:resource="http://www.parameter_estimation_ontology.org#mathematical_function"/>
        <rdfs:range rdf:resource="http://purl.obolibrary.org/obo/IAO_0000029"/>
        <obo:IAO_0000115 xml:lang="en">A relation between a mathematical function and a numeral that represents a correlation matrix where the latter serves as an input to the former.</obo:IAO_0000115>
        <obo:IAO_0000117 xml:lang="en">PERSON: Alexander Klawonn</obo:IAO_0000117>
        <rdfs:label xml:lang="en">has covariance matrix</rdfs:label>
    </owl:ObjectProperty>
    


    <!-- http://www.parameter_estimation_ontology.org#has_data_generation_model -->

    <owl:ObjectProperty rdf:about="http://www.parameter_estimation_ontology.org#has_data_generation_model">
        <rdfs:subPropertyOf rdf:resource="http://purl.obolibrary.org/obo/BFO_0000051"/>
        <rdfs:domain rdf:resource="http://www.parameter_estimation_ontology.org#inverse_problem"/>
        <rdfs:range rdf:resource="http://www.parameter_estimation_ontology.org#data_generation_model"/>
        <obo:IAO_0000115 xml:lang="en">A relation between an inverse problem and a data generation model indicating that the latter is part of the definition of the former.</obo:IAO_0000115>
        <obo:IAO_0000117 xml:lang="en">PERSON: Alexander Klawonn</obo:IAO_0000117>
        <rdfs:label xml:lang="en">has data generation model</rdfs:label>
    </owl:ObjectProperty>
    


    <!-- http://www.parameter_estimation_ontology.org#has_domain -->

    <owl:ObjectProperty rdf:about="http://www.parameter_estimation_ontology.org#has_domain">
        <rdfs:subPropertyOf rdf:resource="http://purl.obolibrary.org/obo/BFO_0000051"/>
        <owl:inverseOf rdf:resource="http://www.parameter_estimation_ontology.org#is_domain_of"/>
        <rdfs:domain rdf:resource="http://www.parameter_estimation_ontology.org#variable"/>
        <rdfs:range rdf:resource="http://www.parameter_estimation_ontology.org#numeric_domain"/>
        <obo:IAO_0000115 xml:lang="en">A relation between a variable and a numeric domain where the latter describes the possible values the former can assume.</obo:IAO_0000115>
        <obo:IAO_0000117 xml:lang="en">PERSON: Alexander Klawonn</obo:IAO_0000117>
        <rdfs:label xml:lang="en">has domain</rdfs:label>
    </owl:ObjectProperty>
    


    <!-- http://www.parameter_estimation_ontology.org#has_experiment -->

    <owl:ObjectProperty rdf:about="http://www.parameter_estimation_ontology.org#has_experiment">
        <rdfs:subPropertyOf rdf:resource="http://purl.obolibrary.org/obo/BFO_0000051"/>
        <rdfs:domain rdf:resource="http://www.parameter_estimation_ontology.org#inverse_problem"/>
        <rdfs:range rdf:resource="http://www.parameter_estimation_ontology.org#single_experiment_data_set"/>
        <obo:IAO_0000115 xml:lang="en">A relation between an inverse problem and an experiment indicating that the latter is part of the definition of the former.</obo:IAO_0000115>
        <obo:IAO_0000117 xml:lang="en">PERSON: Alexander Klawonn</obo:IAO_0000117>
        <rdfs:label xml:lang="en">has experiment</rdfs:label>
    </owl:ObjectProperty>
    


    <!-- http://www.parameter_estimation_ontology.org#has_factor -->

    <owl:ObjectProperty rdf:about="http://www.parameter_estimation_ontology.org#has_factor">
        <rdfs:subPropertyOf rdf:resource="http://www.parameter_estimation_ontology.org#has_argument"/>
        <rdfs:domain rdf:resource="http://www.parameter_estimation_ontology.org#multiplication"/>
        <rdfs:range rdf:resource="http://purl.obolibrary.org/obo/IAO_0000029"/>
        <obo:IAO_0000115 xml:lang="en">A relation between a multiplication and a numeral where the latter serves as an input to the former.</obo:IAO_0000115>
        <obo:IAO_0000117 xml:lang="en">PERSON: Alexander Klawonn</obo:IAO_0000117>
        <rdfs:label xml:lang="en">has factor</rdfs:label>
    </owl:ObjectProperty>
    


    <!-- http://www.parameter_estimation_ontology.org#has_forward_model -->

    <owl:ObjectProperty rdf:about="http://www.parameter_estimation_ontology.org#has_forward_model">
        <rdfs:subPropertyOf rdf:resource="http://purl.obolibrary.org/obo/BFO_0000051"/>
        <rdfs:domain rdf:resource="http://www.parameter_estimation_ontology.org#inverse_problem"/>
        <rdfs:range rdf:resource="http://www.parameter_estimation_ontology.org#forward_model"/>
        <obo:IAO_0000115 xml:lang="en">A relation between an inverse problem and a forward model indicating that the latter is part of the definition of the former.</obo:IAO_0000115>
        <obo:IAO_0000117 xml:lang="en">PERSON: Alexander Klawonn</obo:IAO_0000117>
        <rdfs:label xml:lang="en">has forward model</rdfs:label>
    </owl:ObjectProperty>
    


    <!-- http://www.parameter_estimation_ontology.org#has_input_sensor -->

    <owl:ObjectProperty rdf:about="http://www.parameter_estimation_ontology.org#has_input_sensor">
        <rdfs:subPropertyOf rdf:resource="http://www.parameter_estimation_ontology.org#has_argument"/>
        <rdfs:domain rdf:resource="http://www.parameter_estimation_ontology.org#forward_model"/>
        <rdfs:range rdf:resource="http://www.parameter_estimation_ontology.org#input_sensor"/>
        <obo:IAO_0000115 xml:lang="en">A relation between a forward model and an input sensor where the latter severes as an input to the former.</obo:IAO_0000115>
        <obo:IAO_0000117 xml:lang="en">PERSON: Alexander Klawonn</obo:IAO_0000117>
        <rdfs:label xml:lang="en">has input sensor</rdfs:label>
    </owl:ObjectProperty>
    


    <!-- http://www.parameter_estimation_ontology.org#has_joint_posterior_distribution -->

    <owl:ObjectProperty rdf:about="http://www.parameter_estimation_ontology.org#has_joint_posterior_distribution">
        <rdfs:subPropertyOf rdf:resource="http://purl.obolibrary.org/obo/BFO_0000051"/>
        <rdfs:domain rdf:resource="http://www.parameter_estimation_ontology.org#inverse_problem"/>
        <rdfs:range rdf:resource="http://www.parameter_estimation_ontology.org#probability_distribution_function"/>
        <obo:IAO_0000115 xml:lang="en">A relation between an inverse problem and a probability distribution function where the latter is the result of the inference step with regard to the former.</obo:IAO_0000115>
        <obo:IAO_0000117 xml:lang="en">PERSON: Alexander Klawonn</obo:IAO_0000117>
        <rdfs:label xml:lang="en">has joint posterior distribution</rdfs:label>
    </owl:ObjectProperty>
    


    <!-- http://www.parameter_estimation_ontology.org#has_lower_bound -->

    <owl:ObjectProperty rdf:about="http://www.parameter_estimation_ontology.org#has_lower_bound">
        <rdfs:subPropertyOf rdf:resource="http://www.parameter_estimation_ontology.org#has_argument"/>
        <rdfs:domain rdf:resource="http://www.parameter_estimation_ontology.org#mathematical_function"/>
        <rdfs:range rdf:resource="http://purl.obolibrary.org/obo/IAO_0000029"/>
        <obo:IAO_0000115 xml:lang="en">A relation between a mathematical function and a numeral that represents a lower bound where the latter serves as an input to the former.</obo:IAO_0000115>
        <obo:IAO_0000117 xml:lang="en">PERSON: Alexander Klawonn</obo:IAO_0000117>
        <rdfs:label xml:lang="en">has lower bound</rdfs:label>
    </owl:ObjectProperty>
    


    <!-- http://www.parameter_estimation_ontology.org#has_maximum_likelihood_estimate -->

    <owl:ObjectProperty rdf:about="http://www.parameter_estimation_ontology.org#has_maximum_likelihood_estimate">
        <rdfs:domain rdf:resource="http://www.parameter_estimation_ontology.org#parameter"/>
        <rdfs:range rdf:resource="http://www.parameter_estimation_ontology.org#constant"/>
        <obo:IAO_0000115 xml:lang="en">A relation between a parameter and a constant where the latter describes the maximum likelihood fit of the former.</obo:IAO_0000115>
        <obo:IAO_0000117 xml:lang="en">PERSON: Alexander Klawonn</obo:IAO_0000117>
        <rdfs:label xml:lang="en">has maximum likelihood estimate</rdfs:label>
    </owl:ObjectProperty>
    


    <!-- http://www.parameter_estimation_ontology.org#has_mean -->

    <owl:ObjectProperty rdf:about="http://www.parameter_estimation_ontology.org#has_mean">
        <rdfs:subPropertyOf rdf:resource="http://www.parameter_estimation_ontology.org#has_argument"/>
        <rdfs:domain rdf:resource="http://www.parameter_estimation_ontology.org#mathematical_function"/>
        <rdfs:range rdf:resource="http://purl.obolibrary.org/obo/IAO_0000029"/>
        <obo:IAO_0000115 xml:lang="en">A relation between a mathematical function and a numeral that represents a mean value where the latter serves as an input to the former.</obo:IAO_0000115>
        <obo:IAO_0000117 xml:lang="en">PERSON: Alexander Klawonn</obo:IAO_0000117>
        <rdfs:label xml:lang="en">has mean</rdfs:label>
    </owl:ObjectProperty>
    


    <!-- http://www.parameter_estimation_ontology.org#has_measured_values -->

    <owl:ObjectProperty rdf:about="http://www.parameter_estimation_ontology.org#has_measured_values">
        <rdfs:domain rdf:resource="http://www.parameter_estimation_ontology.org#single_experiment_data_set"/>
        <rdfs:range rdf:resource="http://www.parameter_estimation_ontology.org#constant"/>
        <obo:IAO_0000115 xml:lang="en">A relation between a single experiment data set and a constant where the latter describes some data recoreded by a sensor of the former.</obo:IAO_0000115>
        <obo:IAO_0000117 xml:lang="en">PERSON: Alexander Klawonn</obo:IAO_0000117>
        <rdfs:label xml:lang="en">has measured values</rdfs:label>
    </owl:ObjectProperty>
    


    <!-- http://www.parameter_estimation_ontology.org#has_output_sensor -->

    <owl:ObjectProperty rdf:about="http://www.parameter_estimation_ontology.org#has_output_sensor">
        <rdfs:subPropertyOf rdf:resource="http://www.parameter_estimation_ontology.org#returns"/>
        <rdfs:domain rdf:resource="http://www.parameter_estimation_ontology.org#forward_model"/>
        <rdfs:range rdf:resource="http://www.parameter_estimation_ontology.org#output_sensor"/>
        <obo:IAO_0000115 xml:lang="en">A relation between a forward model and an output sensor where the latter is returned as an output from the former.</obo:IAO_0000115>
        <obo:IAO_0000117 xml:lang="en">PERSON: Alexander Klawonn</obo:IAO_0000117>
        <rdfs:label xml:lang="en">has output sensor</rdfs:label>
    </owl:ObjectProperty>
    


    <!-- http://www.parameter_estimation_ontology.org#has_parameter -->

    <owl:ObjectProperty rdf:about="http://www.parameter_estimation_ontology.org#has_parameter">
        <rdfs:subPropertyOf rdf:resource="http://purl.obolibrary.org/obo/BFO_0000051"/>
        <rdfs:domain rdf:resource="http://www.parameter_estimation_ontology.org#inverse_problem"/>
        <rdfs:range rdf:resource="http://www.parameter_estimation_ontology.org#parameter"/>
        <obo:IAO_0000115 xml:lang="en">A relation between an inverse problem and a parameter indicating that the latter is part of the definition of the former.</obo:IAO_0000115>
        <obo:IAO_0000117 xml:lang="en">PERSON: Alexander Klawonn</obo:IAO_0000117>
        <rdfs:label xml:lang="en">has parameter</rdfs:label>
    </owl:ObjectProperty>
    


    <!-- http://www.parameter_estimation_ontology.org#has_posterior_distribution -->

    <owl:ObjectProperty rdf:about="http://www.parameter_estimation_ontology.org#has_posterior_distribution">
        <rdfs:subPropertyOf rdf:resource="http://purl.obolibrary.org/obo/BFO_0000051"/>
        <owl:inverseOf rdf:resource="http://www.parameter_estimation_ontology.org#is_posterior_distribution_of"/>
        <rdfs:domain rdf:resource="http://www.parameter_estimation_ontology.org#parameter"/>
        <rdfs:range rdf:resource="http://www.parameter_estimation_ontology.org#probability_distribution_function"/>
        <obo:IAO_0000115 xml:lang="en">A relation between a parameter and a probability distribution function where the latter describes the belief of the parameter&apos;s value after inference.</obo:IAO_0000115>
        <obo:IAO_0000117 xml:lang="en">PERSON: Alexander Klawonn</obo:IAO_0000117>
        <rdfs:label xml:lang="en">has posterior distribution</rdfs:label>
    </owl:ObjectProperty>
    


    <!-- http://www.parameter_estimation_ontology.org#has_primary_variable -->

    <owl:ObjectProperty rdf:about="http://www.parameter_estimation_ontology.org#has_primary_variable">
        <rdfs:subPropertyOf rdf:resource="http://www.parameter_estimation_ontology.org#has_argument"/>
        <rdfs:domain rdf:resource="http://www.parameter_estimation_ontology.org#mathematical_function"/>
        <rdfs:range rdf:resource="http://www.parameter_estimation_ontology.org#variable"/>
        <obo:IAO_0000115 xml:lang="en">A relation between a mathematical function and a variable where the latter serves as an input of primary concern to the former.</obo:IAO_0000115>
        <obo:IAO_0000117 xml:lang="en">PERSON: Alexander Klawonn</obo:IAO_0000117>
        <rdfs:label xml:lang="en">has primary variable</rdfs:label>
    </owl:ObjectProperty>
    


    <!-- http://www.parameter_estimation_ontology.org#has_prior_distribution -->

    <owl:ObjectProperty rdf:about="http://www.parameter_estimation_ontology.org#has_prior_distribution">
        <rdfs:subPropertyOf rdf:resource="http://purl.obolibrary.org/obo/BFO_0000051"/>
        <owl:inverseOf rdf:resource="http://www.parameter_estimation_ontology.org#is_prior_distribution_of"/>
        <rdfs:domain rdf:resource="http://www.parameter_estimation_ontology.org#parameter"/>
        <rdfs:range rdf:resource="http://www.parameter_estimation_ontology.org#probability_distribution_function"/>
        <obo:IAO_0000115 xml:lang="en">A relation between a parameter and a probability distribution function where the latter describes the belief of the parameter&apos;s value before inference.</obo:IAO_0000115>
        <obo:IAO_0000117 xml:lang="en">PERSON: Alexander Klawonn</obo:IAO_0000117>
        <rdfs:label xml:lang="en">has prior distribution</rdfs:label>
    </owl:ObjectProperty>
    


    <!-- http://www.parameter_estimation_ontology.org#has_samples -->

    <owl:ObjectProperty rdf:about="http://www.parameter_estimation_ontology.org#has_samples">
        <rdfs:subPropertyOf rdf:resource="http://www.parameter_estimation_ontology.org#has_argument"/>
        <rdfs:domain rdf:resource="http://www.parameter_estimation_ontology.org#mathematical_function"/>
        <rdfs:range rdf:resource="http://www.parameter_estimation_ontology.org#constant"/>
        <obo:IAO_0000115 xml:lang="en">A relation between a mathematical function and a constant where the latter is used as an input to the former.</obo:IAO_0000115>
        <obo:IAO_0000117 xml:lang="en">PERSON: Alexander Klawonn</obo:IAO_0000117>
        <rdfs:label xml:lang="en">has samples</rdfs:label>
    </owl:ObjectProperty>
    


    <!-- http://www.parameter_estimation_ontology.org#has_sensor -->

    <owl:ObjectProperty rdf:about="http://www.parameter_estimation_ontology.org#has_sensor">
        <rdfs:domain rdf:resource="http://www.parameter_estimation_ontology.org#single_experiment_data_set"/>
        <rdfs:range rdf:resource="http://www.parameter_estimation_ontology.org#sensor"/>
        <obo:IAO_0000115 xml:lang="en">A relation between a single experiment data set and a sensor where the latter is part of the former.</obo:IAO_0000115>
        <obo:IAO_0000117 xml:lang="en">PERSON: Alexander Klawonn</obo:IAO_0000117>
        <rdfs:label xml:lang="en">has sensor</rdfs:label>
    </owl:ObjectProperty>
    


    <!-- http://www.parameter_estimation_ontology.org#has_standard_deviation -->

    <owl:ObjectProperty rdf:about="http://www.parameter_estimation_ontology.org#has_standard_deviation">
        <rdfs:subPropertyOf rdf:resource="http://www.parameter_estimation_ontology.org#has_argument"/>
        <rdfs:domain rdf:resource="http://www.parameter_estimation_ontology.org#mathematical_function"/>
        <rdfs:range rdf:resource="http://purl.obolibrary.org/obo/IAO_0000029"/>
        <obo:IAO_0000115 xml:lang="en">A relation between a mathematical function and a numeral that represents a standard deviation where the latter serves as an input to the former.</obo:IAO_0000115>
        <obo:IAO_0000117 xml:lang="en">PERSON: Alexander Klawonn</obo:IAO_0000117>
        <rdfs:label xml:lang="en">has standard deviation</rdfs:label>
    </owl:ObjectProperty>
    


    <!-- http://www.parameter_estimation_ontology.org#has_summand -->

    <owl:ObjectProperty rdf:about="http://www.parameter_estimation_ontology.org#has_summand">
        <rdfs:subPropertyOf rdf:resource="http://www.parameter_estimation_ontology.org#has_argument"/>
        <rdfs:domain rdf:resource="http://www.parameter_estimation_ontology.org#addition"/>
        <rdfs:range rdf:resource="http://purl.obolibrary.org/obo/IAO_0000029"/>
        <obo:IAO_0000115 xml:lang="en">A relation between an addition and a numeral where the latter serves as an input to a sum in the former.</obo:IAO_0000115>
        <obo:IAO_0000117 xml:lang="en">PERSON: Alexander Klawonn</obo:IAO_0000117>
        <rdfs:label xml:lang="en">has summand</rdfs:label>
    </owl:ObjectProperty>
    


    <!-- http://www.parameter_estimation_ontology.org#has_upper_bound -->

    <owl:ObjectProperty rdf:about="http://www.parameter_estimation_ontology.org#has_upper_bound">
        <rdfs:subPropertyOf rdf:resource="http://www.parameter_estimation_ontology.org#has_argument"/>
        <rdfs:domain rdf:resource="http://www.parameter_estimation_ontology.org#mathematical_function"/>
        <rdfs:range rdf:resource="http://purl.obolibrary.org/obo/IAO_0000029"/>
        <obo:IAO_0000115 xml:lang="en">A relation between a mathematical function and a numeral that represents an upper bound where the latter serves as an input to the former.</obo:IAO_0000115>
        <obo:IAO_0000117 xml:lang="en">PERSON: Alexander Klawonn</obo:IAO_0000117>
        <rdfs:label xml:lang="en">has upper bound</rdfs:label>
    </owl:ObjectProperty>
    


    <!-- http://www.parameter_estimation_ontology.org#is_deterministically_modeled_by -->

    <owl:ObjectProperty rdf:about="http://www.parameter_estimation_ontology.org#is_deterministically_modeled_by">
        <rdfs:domain rdf:resource="http://www.parameter_estimation_ontology.org#single_experiment_data_set"/>
        <rdfs:range rdf:resource="http://www.parameter_estimation_ontology.org#forward_model"/>
        <obo:IAO_0000115 xml:lang="en">A relation between a single experiment data set and a forward model where the latter describes some part of the data of the former in deterministic terms (i.e., without considering uncertainty).</obo:IAO_0000115>
        <obo:IAO_0000117 xml:lang="en">PERSON: Alexander Klawonn</obo:IAO_0000117>
        <rdfs:label xml:lang="en">is deterministically modeled by</rdfs:label>
    </owl:ObjectProperty>
    


    <!-- http://www.parameter_estimation_ontology.org#is_domain_of -->

    <owl:ObjectProperty rdf:about="http://www.parameter_estimation_ontology.org#is_domain_of">
        <rdfs:subPropertyOf rdf:resource="http://purl.obolibrary.org/obo/BFO_0000050"/>
        <rdfs:domain rdf:resource="http://www.parameter_estimation_ontology.org#numeric_domain"/>
        <rdfs:range rdf:resource="http://www.parameter_estimation_ontology.org#variable"/>
        <obo:IAO_0000115 xml:lang="en">A relation between a numeric domain and a variable where the former describes the possible values the latter can assume.</obo:IAO_0000115>
        <obo:IAO_0000117 xml:lang="en">PERSON: Alexander Klawonn</obo:IAO_0000117>
        <rdfs:label xml:lang="en">is domain of</rdfs:label>
    </owl:ObjectProperty>
    


    <!-- http://www.parameter_estimation_ontology.org#is_posterior_distribution_of -->

    <owl:ObjectProperty rdf:about="http://www.parameter_estimation_ontology.org#is_posterior_distribution_of">
        <rdfs:subPropertyOf rdf:resource="http://purl.obolibrary.org/obo/BFO_0000050"/>
        <rdfs:domain rdf:resource="http://www.parameter_estimation_ontology.org#probability_distribution_function"/>
        <rdfs:range rdf:resource="http://www.parameter_estimation_ontology.org#parameter"/>
        <obo:IAO_0000115 xml:lang="en">A relation between a probability distribution function and a parameter where the former describes the belief of the parameter&apos;s value after inference.</obo:IAO_0000115>
        <obo:IAO_0000117 xml:lang="en">PERSON: Alexander Klawonn</obo:IAO_0000117>
        <rdfs:label xml:lang="en">is posterior distribution of</rdfs:label>
    </owl:ObjectProperty>
    


    <!-- http://www.parameter_estimation_ontology.org#is_prior_distribution_of -->

    <owl:ObjectProperty rdf:about="http://www.parameter_estimation_ontology.org#is_prior_distribution_of">
        <rdfs:subPropertyOf rdf:resource="http://purl.obolibrary.org/obo/BFO_0000050"/>
        <rdfs:domain rdf:resource="http://www.parameter_estimation_ontology.org#probability_distribution_function"/>
        <rdfs:range rdf:resource="http://www.parameter_estimation_ontology.org#parameter"/>
        <obo:IAO_0000115 xml:lang="en">A relation between a probability distribution function and a parameter where the former describes the belief of the parameter&apos;s value before inference.</obo:IAO_0000115>
        <obo:IAO_0000117 xml:lang="en">PERSON: Alexander Klawonn</obo:IAO_0000117>
        <rdfs:label xml:lang="en">is prior distribution of</rdfs:label>
    </owl:ObjectProperty>
    


    <!-- http://www.parameter_estimation_ontology.org#is_stochastically_modeled_by -->

    <owl:ObjectProperty rdf:about="http://www.parameter_estimation_ontology.org#is_stochastically_modeled_by">
        <owl:inverseOf rdf:resource="http://www.parameter_estimation_ontology.org#stochastically_models_experiment"/>
        <rdfs:domain rdf:resource="http://www.parameter_estimation_ontology.org#single_experiment_data_set"/>
        <rdfs:range rdf:resource="http://purl.obolibrary.org/obo/IAO_0000029"/>
        <obo:IAO_0000115 xml:lang="en">A relation between a single experiment data set and a data generation model where the latter describes some part of the data of the former in stochastic terms.</obo:IAO_0000115>
        <obo:IAO_0000117 xml:lang="en">PERSON: Alexander Klawonn</obo:IAO_0000117>
        <rdfs:label xml:lang="en">is stochastically modeled by</rdfs:label>
    </owl:ObjectProperty>
    


    <!-- http://www.parameter_estimation_ontology.org#is_used_by_mathematical_function -->

    <owl:ObjectProperty rdf:about="http://www.parameter_estimation_ontology.org#is_used_by_mathematical_function">
        <owl:inverseOf rdf:resource="http://www.parameter_estimation_ontology.org#uses_mathematical_function"/>
        <rdf:type rdf:resource="http://www.w3.org/2002/07/owl#AsymmetricProperty"/>
        <rdfs:domain rdf:resource="http://www.parameter_estimation_ontology.org#mathematical_function"/>
        <rdfs:range rdf:resource="http://www.parameter_estimation_ontology.org#mathematical_function"/>
        <obo:IAO_0000115 xml:lang="en">A relation between a mathematical function and another mathematical function that indicates that the former is used by the latter in its computations.</obo:IAO_0000115>
        <obo:IAO_0000117 xml:lang="en">PERSON: Alexander Klawonn</obo:IAO_0000117>
        <rdfs:label xml:lang="en">is used by mathematical function</rdfs:label>
    </owl:ObjectProperty>
    


    <!-- http://www.parameter_estimation_ontology.org#model_error_scatter_described_by -->

    <owl:ObjectProperty rdf:about="http://www.parameter_estimation_ontology.org#model_error_scatter_described_by">
        <rdfs:domain rdf:resource="http://www.parameter_estimation_ontology.org#output_sensor"/>
        <rdfs:range rdf:resource="http://purl.obolibrary.org/obo/IAO_0000029"/>
        <obo:IAO_0000115 xml:lang="en">A relation between an output sensor and a numeral where the latter describes the scatter (for example the standard deviation) of the difference between the model prediction returned by the output sensor and the corresponding experimental data.</obo:IAO_0000115>
        <obo:IAO_0000117 xml:lang="en">PERSON: Alexander Klawonn</obo:IAO_0000117>
        <rdfs:label xml:lang="en">model error scatter described by</rdfs:label>
    </owl:ObjectProperty>
    


    <!-- http://www.parameter_estimation_ontology.org#returns -->

    <owl:ObjectProperty rdf:about="http://www.parameter_estimation_ontology.org#returns">
        <rdfs:domain rdf:resource="http://www.parameter_estimation_ontology.org#mathematical_function"/>
        <rdfs:range rdf:resource="http://purl.obolibrary.org/obo/IAO_0000029"/>
        <obo:IAO_0000115 xml:lang="en">A relation between a mathematical function and a numeral where the latter is returned as an output from the former.</obo:IAO_0000115>
        <obo:IAO_0000117 xml:lang="en">PERSON: Alexander Klawonn</obo:IAO_0000117>
        <rdfs:label xml:lang="en">returns</rdfs:label>
    </owl:ObjectProperty>
    


    <!-- http://www.parameter_estimation_ontology.org#stochastically_models_experiment -->

    <owl:ObjectProperty rdf:about="http://www.parameter_estimation_ontology.org#stochastically_models_experiment">
        <rdfs:domain rdf:resource="http://www.parameter_estimation_ontology.org#data_generation_model"/>
        <rdfs:range rdf:resource="http://www.parameter_estimation_ontology.org#single_experiment_data_set"/>
        <obo:IAO_0000115 xml:lang="en">A relation between a data generation model and a single experiment data set where the former describes some part of the data of the latter in stochastic terms.</obo:IAO_0000115>
        <obo:IAO_0000117 xml:lang="en">PERSON: Alexander Klawonn</obo:IAO_0000117>
        <rdfs:label xml:lang="en">stochastically models experiment</rdfs:label>
    </owl:ObjectProperty>
    


    <!-- http://www.parameter_estimation_ontology.org#uses_mathematical_function -->

    <owl:ObjectProperty rdf:about="http://www.parameter_estimation_ontology.org#uses_mathematical_function">
        <rdf:type rdf:resource="http://www.w3.org/2002/07/owl#AsymmetricProperty"/>
        <rdfs:domain rdf:resource="http://www.parameter_estimation_ontology.org#mathematical_function"/>
        <rdfs:range rdf:resource="http://www.parameter_estimation_ontology.org#mathematical_function"/>
        <obo:IAO_0000115 xml:lang="en">A relation between a mathematical function and another mathematical function that indicates that the former is using the latter in its computations.</obo:IAO_0000115>
        <obo:IAO_0000117 xml:lang="en">PERSON: Alexander Klawonn</obo:IAO_0000117>
        <rdfs:label xml:lang="en">uses mathematical function</rdfs:label>
    </owl:ObjectProperty>
    


    <!-- 
    ///////////////////////////////////////////////////////////////////////////////////////
    //
    // Data properties
    //
    ///////////////////////////////////////////////////////////////////////////////////////
     -->

    


    <!-- http://www.parameter_estimation_ontology.org#has_dimension -->

    <owl:DatatypeProperty rdf:about="http://www.parameter_estimation_ontology.org#has_dimension">
        <rdfs:domain rdf:resource="http://purl.obolibrary.org/obo/IAO_0000029"/>
        <rdfs:range rdf:resource="http://www.w3.org/2001/XMLSchema#positiveInteger"/>
        <obo:IAO_0000117 xml:lang="en">PERSON: Alexander Klawonn</obo:IAO_0000117>
        <rdfs:label xml:lang="en">has dimension</rdfs:label>
    </owl:DatatypeProperty>
    


    <!-- http://www.parameter_estimation_ontology.org#has_explanation -->

    <owl:DatatypeProperty rdf:about="http://www.parameter_estimation_ontology.org#has_explanation">
        <rdfs:domain rdf:resource="http://purl.obolibrary.org/obo/IAO_0000029"/>
        <rdfs:range rdf:resource="http://www.w3.org/2001/XMLSchema#string"/>
        <obo:IAO_0000117 xml:lang="en">PERSON: Alexander Klawonn</obo:IAO_0000117>
        <rdfs:label xml:lang="en">has explanation</rdfs:label>
    </owl:DatatypeProperty>
    


    <!-- http://www.parameter_estimation_ontology.org#has_file -->

    <owl:DatatypeProperty rdf:about="http://www.parameter_estimation_ontology.org#has_file">
        <rdfs:domain rdf:resource="http://www.parameter_estimation_ontology.org#constant"/>
        <rdfs:range rdf:resource="http://www.w3.org/2001/XMLSchema#string"/>
        <obo:IAO_0000117 xml:lang="en">PERSON: Alexander Klawonn</obo:IAO_0000117>
        <rdfs:label xml:lang="en">has file</rdfs:label>
    </owl:DatatypeProperty>
    


    <!-- http://www.parameter_estimation_ontology.org#has_index -->

    <owl:DatatypeProperty rdf:about="http://www.parameter_estimation_ontology.org#has_index">
        <rdfs:domain rdf:resource="http://www.parameter_estimation_ontology.org#numeric_domain"/>
        <rdfs:range rdf:resource="http://www.w3.org/2001/XMLSchema#nonNegativeInteger"/>
        <obo:IAO_0000117 xml:lang="en">PERSON: Alexander Klawonn</obo:IAO_0000117>
        <rdfs:label xml:lang="en">has index</rdfs:label>
    </owl:DatatypeProperty>
    


    <!-- http://www.parameter_estimation_ontology.org#has_lower_bound_value -->

    <owl:DatatypeProperty rdf:about="http://www.parameter_estimation_ontology.org#has_lower_bound_value">
        <rdfs:domain rdf:resource="http://www.parameter_estimation_ontology.org#one_dimensional_interval"/>
        <rdfs:range rdf:resource="http://www.w3.org/2001/XMLSchema#float"/>
        <obo:IAO_0000117 xml:lang="en">PERSON: Alexander Klawonn</obo:IAO_0000117>
        <rdfs:label xml:lang="en">has lower bound value</rdfs:label>
    </owl:DatatypeProperty>
    


    <!-- http://www.parameter_estimation_ontology.org#has_number_of_columns -->

    <owl:DatatypeProperty rdf:about="http://www.parameter_estimation_ontology.org#has_number_of_columns">
        <rdfs:domain rdf:resource="http://www.parameter_estimation_ontology.org#constant"/>
        <rdfs:range rdf:resource="http://www.w3.org/2001/XMLSchema#nonPositiveInteger"/>
        <obo:IAO_0000117 xml:lang="en">PERSON: Alexander Klawonn</obo:IAO_0000117>
        <rdfs:label xml:lang="en">has number of columns</rdfs:label>
    </owl:DatatypeProperty>
    


    <!-- http://www.parameter_estimation_ontology.org#has_number_of_rows -->

    <owl:DatatypeProperty rdf:about="http://www.parameter_estimation_ontology.org#has_number_of_rows">
        <rdfs:domain rdf:resource="http://www.parameter_estimation_ontology.org#constant"/>
        <rdfs:range rdf:resource="http://www.w3.org/2001/XMLSchema#nonPositiveInteger"/>
        <obo:IAO_0000117 xml:lang="en">PERSON: Alexander Klawonn</obo:IAO_0000117>
        <rdfs:label xml:lang="en">has number of rows</rdfs:label>
    </owl:DatatypeProperty>
    


    <!-- http://www.parameter_estimation_ontology.org#has_posterior_index -->

    <owl:DatatypeProperty rdf:about="http://www.parameter_estimation_ontology.org#has_posterior_index">
        <rdfs:domain rdf:resource="http://www.parameter_estimation_ontology.org#parameter"/>
        <rdfs:range rdf:resource="http://www.w3.org/2001/XMLSchema#nonNegativeInteger"/>
        <obo:IAO_0000117 xml:lang="en">PERSON: Alexander Klawonn</obo:IAO_0000117>
        <rdfs:label xml:lang="en">has posterior index</rdfs:label>
    </owl:DatatypeProperty>
    


    <!-- http://www.parameter_estimation_ontology.org#has_scalar_value -->

    <owl:DatatypeProperty rdf:about="http://www.parameter_estimation_ontology.org#has_scalar_value">
        <rdfs:domain rdf:resource="http://www.parameter_estimation_ontology.org#scalar_constant"/>
        <rdfs:range rdf:resource="http://www.w3.org/2001/XMLSchema#float"/>
        <obo:IAO_0000117 xml:lang="en">PERSON: Alexander Klawonn</obo:IAO_0000117>
        <rdfs:label xml:lang="en">has scalar value</rdfs:label>
    </owl:DatatypeProperty>
    


    <!-- http://www.parameter_estimation_ontology.org#has_tex_symbol -->

    <owl:DatatypeProperty rdf:about="http://www.parameter_estimation_ontology.org#has_tex_symbol">
        <rdfs:domain rdf:resource="http://purl.obolibrary.org/obo/IAO_0000029"/>
        <rdfs:range rdf:resource="http://www.w3.org/2001/XMLSchema#string"/>
        <obo:IAO_0000117 xml:lang="en">PERSON: Alexander Klawonn</obo:IAO_0000117>
        <rdfs:label xml:lang="en">has tex symbol</rdfs:label>
    </owl:DatatypeProperty>
    


    <!-- http://www.parameter_estimation_ontology.org#has_upper_bound_value -->

    <owl:DatatypeProperty rdf:about="http://www.parameter_estimation_ontology.org#has_upper_bound_value">
        <rdfs:domain rdf:resource="http://www.parameter_estimation_ontology.org#one_dimensional_interval"/>
        <rdfs:range rdf:resource="http://www.w3.org/2001/XMLSchema#float"/>
        <obo:IAO_0000117 xml:lang="en">PERSON: Alexander Klawonn</obo:IAO_0000117>
        <rdfs:label xml:lang="en">has upper bound value</rdfs:label>
    </owl:DatatypeProperty>
    


    <!-- http://www.parameter_estimation_ontology.org#lower_bound_included -->

    <owl:DatatypeProperty rdf:about="http://www.parameter_estimation_ontology.org#lower_bound_included">
        <rdfs:domain rdf:resource="http://www.parameter_estimation_ontology.org#one_dimensional_interval"/>
        <rdfs:range rdf:resource="http://www.w3.org/2001/XMLSchema#boolean"/>
        <obo:IAO_0000117 xml:lang="en">PERSON: Alexander Klawonn</obo:IAO_0000117>
        <rdfs:label xml:lang="en">lower bound included</rdfs:label>
    </owl:DatatypeProperty>
    


    <!-- http://www.parameter_estimation_ontology.org#upper_bound_included -->

    <owl:DatatypeProperty rdf:about="http://www.parameter_estimation_ontology.org#upper_bound_included">
        <rdfs:domain rdf:resource="http://www.parameter_estimation_ontology.org#one_dimensional_interval"/>
        <rdfs:range rdf:resource="http://www.w3.org/2001/XMLSchema#boolean"/>
        <obo:IAO_0000117 xml:lang="en">PERSON: Alexander Klawonn</obo:IAO_0000117>
        <rdfs:label xml:lang="en">upper bound included</rdfs:label>
    </owl:DatatypeProperty>
    


    <!-- 
    ///////////////////////////////////////////////////////////////////////////////////////
    //
    // Classes
    //
    ///////////////////////////////////////////////////////////////////////////////////////
     -->

    


    <!-- http://www.parameter_estimation_ontology.org#addition -->

    <owl:Class rdf:about="http://www.parameter_estimation_ontology.org#addition">
        <rdfs:subClassOf rdf:resource="http://www.parameter_estimation_ontology.org#mathematical_function"/>
        <obo:IAO_0000115 xml:lang="en">A mathematical function that sums up its inputs.</obo:IAO_0000115>
        <obo:IAO_0000117 xml:lang="en">PERSON: Alexander Klawonn</obo:IAO_0000117>
        <rdfs:label xml:lang="en">addition</rdfs:label>
    </owl:Class>
    


    <!-- http://www.parameter_estimation_ontology.org#concatenation -->

    <owl:Class rdf:about="http://www.parameter_estimation_ontology.org#concatenation">
        <rdfs:subClassOf rdf:resource="http://www.parameter_estimation_ontology.org#mathematical_function"/>
        <obo:IAO_0000115 xml:lang="en">A mathematical function that takes vectors as inputs and returns a concatenation of those input vectors.</obo:IAO_0000115>
        <obo:IAO_0000117 xml:lang="en">PERSON: Alexander Klawonn</obo:IAO_0000117>
        <rdfs:label xml:lang="en">concatenation</rdfs:label>
    </owl:Class>
    


    <!-- http://www.parameter_estimation_ontology.org#constant -->

    <owl:Class rdf:about="http://www.parameter_estimation_ontology.org#constant">
        <rdfs:subClassOf rdf:resource="http://purl.obolibrary.org/obo/IAO_0000029"/>
        <obo:IAO_0000115 xml:lang="en">A numeral that specifies the numeric element(s) it denotes by their value(s).</obo:IAO_0000115>
        <obo:IAO_0000117 xml:lang="en">PERSON: Alexander Klawonn</obo:IAO_0000117>
        <rdfs:label xml:lang="en">constant</rdfs:label>
    </owl:Class>
    


    <!-- http://www.parameter_estimation_ontology.org#correlation_function -->

    <owl:Class rdf:about="http://www.parameter_estimation_ontology.org#correlation_function">
        <rdfs:subClassOf rdf:resource="http://www.parameter_estimation_ontology.org#mathematical_function"/>
        <obo:IAO_0000115 xml:lang="en">A mathematical function that is used to model correlation effects.</obo:IAO_0000115>
        <obo:IAO_0000117 xml:lang="en">PERSON: Alexander Klawonn</obo:IAO_0000117>
        <rdfs:label xml:lang="en">correlation function</rdfs:label>
    </owl:Class>
    


    <!-- http://www.parameter_estimation_ontology.org#covariance_matrix_assembler -->

    <owl:Class rdf:about="http://www.parameter_estimation_ontology.org#covariance_matrix_assembler">
        <rdfs:subClassOf rdf:resource="http://www.parameter_estimation_ontology.org#mathematical_function"/>
        <obo:IAO_0000115 xml:lang="en">A mathematical function that computes a covariance matrix.</obo:IAO_0000115>
        <obo:IAO_0000117 xml:lang="en">PERSON: Alexander Klawonn</obo:IAO_0000117>
        <rdfs:label xml:lang="en">covariance matrix assembler</rdfs:label>
    </owl:Class>
    


    <!-- http://www.parameter_estimation_ontology.org#data_generation_model -->

    <owl:Class rdf:about="http://www.parameter_estimation_ontology.org#data_generation_model">
        <rdfs:subClassOf rdf:resource="http://www.parameter_estimation_ontology.org#mathematical_function"/>
        <obo:IAO_0000115 xml:lang="en">A mathematical function that aims to reproduce a given data set not necessarily exactly but in statistical terms.</obo:IAO_0000115>
        <obo:IAO_0000117 xml:lang="en">PERSON: Alexander Klawonn</obo:IAO_0000117>
        <rdfs:label xml:lang="en">data generation model</rdfs:label>
    </owl:Class>
    


    <!-- http://www.parameter_estimation_ontology.org#forward_model -->

    <owl:Class rdf:about="http://www.parameter_estimation_ontology.org#forward_model">
        <rdfs:subClassOf rdf:resource="http://www.parameter_estimation_ontology.org#mathematical_function"/>
        <obo:IAO_0000115 xml:lang="en">A mathematical function that describes the effect of some cause.</obo:IAO_0000115>
        <obo:IAO_0000117 xml:lang="en">PERSON: Alexander Klawonn</obo:IAO_0000117>
        <rdfs:label xml:lang="en">forward model</rdfs:label>
    </owl:Class>
    


    <!-- http://www.parameter_estimation_ontology.org#input_sensor -->

    <owl:Class rdf:about="http://www.parameter_estimation_ontology.org#input_sensor">
        <rdfs:subClassOf rdf:resource="http://www.parameter_estimation_ontology.org#sensor"/>
        <obo:IAO_0000115 xml:lang="en">A sensor that is used as an argument of a forward model.</obo:IAO_0000115>
        <obo:IAO_0000117 xml:lang="en">PERSON: Alexander Klawonn</obo:IAO_0000117>
        <rdfs:label xml:lang="en">input sensor</rdfs:label>
    </owl:Class>
    


    <!-- http://www.parameter_estimation_ontology.org#inverse_problem -->

    <owl:Class rdf:about="http://www.parameter_estimation_ontology.org#inverse_problem">
        <rdfs:subClassOf rdf:resource="http://www.parameter_estimation_ontology.org#mathematical_problem"/>
        <obo:IAO_0000115 xml:lang="en">A mathematical problem that asks for the causes of some observed effect.</obo:IAO_0000115>
        <obo:IAO_0000117 xml:lang="en">PERSON: Alexander Klawonn</obo:IAO_0000117>
        <rdfs:label xml:lang="en">inverse problem</rdfs:label>
    </owl:Class>
    


    <!-- http://www.parameter_estimation_ontology.org#lognormal_density_function -->

    <owl:Class rdf:about="http://www.parameter_estimation_ontology.org#lognormal_density_function">
        <rdfs:subClassOf rdf:resource="http://www.parameter_estimation_ontology.org#probability_density_function"/>
        <obo:IAO_0000115 xml:lang="en">A probability density function that is based on the log-normal distribution.</obo:IAO_0000115>
        <obo:IAO_0000117 xml:lang="en">PERSON: Alexander Klawonn</obo:IAO_0000117>
        <rdfs:label xml:lang="en">log-normal density function</rdfs:label>
    </owl:Class>
    


    <!-- http://www.parameter_estimation_ontology.org#mathematical_function -->

    <owl:Class rdf:about="http://www.parameter_estimation_ontology.org#mathematical_function">
        <rdfs:subClassOf rdf:resource="http://purl.obolibrary.org/obo/IAO_0000064"/>
        <obo:IAO_0000115 xml:lang="en">An algorithm that contains mathematical operations as its action specification.</obo:IAO_0000115>
        <obo:IAO_0000117 xml:lang="en">PERSON: Alexander Klawonn</obo:IAO_0000117>
        <rdfs:label xml:lang="en">mathematical function</rdfs:label>
    </owl:Class>
    


    <!-- http://www.parameter_estimation_ontology.org#mathematical_problem -->

    <owl:Class rdf:about="http://www.parameter_estimation_ontology.org#mathematical_problem">
        <rdfs:subClassOf rdf:resource="http://www.parameter_estimation_ontology.org#problem"/>
        <obo:IAO_0000115 xml:lang="en">A problem the question(s) of which is/are of mathematical nature.</obo:IAO_0000115>
        <obo:IAO_0000117 xml:lang="en">PERSON: Alexander Klawonn</obo:IAO_0000117>
        <rdfs:label xml:lang="en">mathematical problem</rdfs:label>
    </owl:Class>
    


    <!-- http://www.parameter_estimation_ontology.org#multiplication -->

    <owl:Class rdf:about="http://www.parameter_estimation_ontology.org#multiplication">
        <rdfs:subClassOf rdf:resource="http://www.parameter_estimation_ontology.org#mathematical_function"/>
        <obo:IAO_0000115 xml:lang="en">A mathematical function that sums up its inputs.</obo:IAO_0000115>
        <obo:IAO_0000117 xml:lang="en">PERSON: Alexander Klawonn</obo:IAO_0000117>
        <rdfs:label xml:lang="en">multiplication</rdfs:label>
    </owl:Class>
    


    <!-- http://www.parameter_estimation_ontology.org#normal_density_function -->

    <owl:Class rdf:about="http://www.parameter_estimation_ontology.org#normal_density_function">
        <rdfs:subClassOf rdf:resource="http://www.parameter_estimation_ontology.org#probability_density_function"/>
        <obo:IAO_0000115 xml:lang="en">A probability density function that is based on a normal (also called Gaussian) distribution.</obo:IAO_0000115>
        <obo:IAO_0000117 xml:lang="en">PERSON: Alexander Klawonn</obo:IAO_0000117>
        <rdfs:label xml:lang="en">normal density function</rdfs:label>
    </owl:Class>
    


    <!-- http://www.parameter_estimation_ontology.org#normal_random_variable -->

    <owl:Class rdf:about="http://www.parameter_estimation_ontology.org#normal_random_variable">
        <rdfs:subClassOf rdf:resource="http://www.parameter_estimation_ontology.org#random_variable"/>
        <obo:IAO_0000115 xml:lang="en">A random variable the probability distribution of which is normal (Gaussian).</obo:IAO_0000115>
        <obo:IAO_0000117 xml:lang="en">PERSON: Alexander Klawonn</obo:IAO_0000117>
        <rdfs:label xml:lang="en">normal random variable</rdfs:label>
    </owl:Class>
    


    <!-- http://www.parameter_estimation_ontology.org#numeric_domain -->

    <owl:Class rdf:about="http://www.parameter_estimation_ontology.org#numeric_domain">
        <rdfs:subClassOf rdf:resource="http://purl.obolibrary.org/obo/IAO_0000028"/>
        <obo:IAO_0000115 xml:lang="en">A numeral that represents a finite, countable or uncountalbe amount of numeric elements (scalars, vectors, etc.) of the same type.</obo:IAO_0000115>
        <obo:IAO_0000117 xml:lang="en">PERSON: Alexander Klawonn</obo:IAO_0000117>
        <rdfs:label xml:lang="en">numeric domain</rdfs:label>
    </owl:Class>
    


    <!-- http://www.parameter_estimation_ontology.org#one_dimensional_interval -->

    <owl:Class rdf:about="http://www.parameter_estimation_ontology.org#one_dimensional_interval">
        <rdfs:subClassOf rdf:resource="http://www.parameter_estimation_ontology.org#numeric_domain"/>
        <obo:IAO_0000115 xml:lang="en">A numeric domain the numeric elements of which are scalar (i.e., one dimensional) numbers.</obo:IAO_0000115>
        <obo:IAO_0000117 xml:lang="en">PERSON: Alexander Klawonn</obo:IAO_0000117>
        <rdfs:label xml:lang="en">one dimensional interval</rdfs:label>
    </owl:Class>
    


    <!-- http://www.parameter_estimation_ontology.org#output_sensor -->

    <owl:Class rdf:about="http://www.parameter_estimation_ontology.org#output_sensor">
        <rdfs:subClassOf rdf:resource="http://www.parameter_estimation_ontology.org#sensor"/>
        <obo:IAO_0000115 xml:lang="en">A sensor that is returned by a forward model the value of which should be compared to experimentally measured data.</obo:IAO_0000115>
        <obo:IAO_0000117 xml:lang="en">PERSON: Alexander Klawonn</obo:IAO_0000117>
        <rdfs:label xml:lang="en">output sensor</rdfs:label>
    </owl:Class>
    


    <!-- http://www.parameter_estimation_ontology.org#parameter -->

    <owl:Class rdf:about="http://www.parameter_estimation_ontology.org#parameter">
        <rdfs:subClassOf rdf:resource="http://www.parameter_estimation_ontology.org#random_variable"/>
        <obo:IAO_0000115 xml:lang="en">A random variable that has a probability distribution defined on its domain which is interpreted as prior knowledge.</obo:IAO_0000115>
        <obo:IAO_0000117 xml:lang="en">PERSON: Alexander Klawonn</obo:IAO_0000117>
        <rdfs:label xml:lang="en">parameter</rdfs:label>
    </owl:Class>
    


    <!-- http://www.parameter_estimation_ontology.org#probability_density_function -->

    <owl:Class rdf:about="http://www.parameter_estimation_ontology.org#probability_density_function">
        <rdfs:subClassOf rdf:resource="http://www.parameter_estimation_ontology.org#probability_distribution_function"/>
        <obo:IAO_0000115 xml:lang="en">A probability distribution function that returns a probability density.</obo:IAO_0000115>
        <obo:IAO_0000117 xml:lang="en">PERSON: Alexander Klawonn</obo:IAO_0000117>
        <rdfs:label xml:lang="en">probability density function</rdfs:label>
    </owl:Class>
    


    <!-- http://www.parameter_estimation_ontology.org#probability_distribution_function -->

    <owl:Class rdf:about="http://www.parameter_estimation_ontology.org#probability_distribution_function">
        <rdfs:subClassOf rdf:resource="http://www.parameter_estimation_ontology.org#mathematical_function"/>
        <obo:IAO_0000115 xml:lang="en">A mathematical function that results in some measure related to probability.</obo:IAO_0000115>
        <obo:IAO_0000117 xml:lang="en">PERSON: Alexander Klawonn</obo:IAO_0000117>
        <rdfs:label xml:lang="en">probability distribution function</rdfs:label>
    </owl:Class>
    


    <!-- http://www.parameter_estimation_ontology.org#problem -->

    <owl:Class rdf:about="http://www.parameter_estimation_ontology.org#problem">
        <rdfs:subClassOf rdf:resource="http://purl.obolibrary.org/obo/IAO_0000030"/>
        <obo:IAO_0000115 xml:lang="en">An information content entity that comprises one or multiple questions the answers of which are unknown but also of interest.</obo:IAO_0000115>
        <obo:IAO_0000117 xml:lang="en">PERSON: Alexander Klawonn</obo:IAO_0000117>
    </owl:Class>
    


    <!-- http://www.parameter_estimation_ontology.org#random_variable -->

    <owl:Class rdf:about="http://www.parameter_estimation_ontology.org#random_variable">
        <rdfs:subClassOf rdf:resource="http://www.parameter_estimation_ontology.org#variable"/>
        <obo:IAO_0000115 xml:lang="en">A variable that has a probability distribution defined on its domain.</obo:IAO_0000115>
        <obo:IAO_0000117 xml:lang="en">PERSON: Alexander Klawonn</obo:IAO_0000117>
        <rdfs:label xml:lang="en">random variable</rdfs:label>
    </owl:Class>
    


    <!-- http://www.parameter_estimation_ontology.org#sample_based_density_function -->

    <owl:Class rdf:about="http://www.parameter_estimation_ontology.org#sample_based_density_function">
        <rdfs:subClassOf rdf:resource="http://www.parameter_estimation_ontology.org#probability_density_function"/>
        <obo:IAO_0000115 xml:lang="en">A probability density function that is defined by a number of samples.</obo:IAO_0000115>
        <obo:IAO_0000117 xml:lang="en">PERSON: Alexander Klawonn</obo:IAO_0000117>
        <rdfs:label xml:lang="en">sample-based density function</rdfs:label>
    </owl:Class>
    


    <!-- http://www.parameter_estimation_ontology.org#scalar_constant -->

    <owl:Class rdf:about="http://www.parameter_estimation_ontology.org#scalar_constant">
        <rdfs:subClassOf rdf:resource="http://www.parameter_estimation_ontology.org#constant"/>
        <obo:IAO_0000115 xml:lang="en">A constant that represents exactly one number.</obo:IAO_0000115>
        <obo:IAO_0000117 xml:lang="en">PERSON: Alexander Klawonn</obo:IAO_0000117>
        <rdfs:label xml:lang="en">scalar constant</rdfs:label>
    </owl:Class>
    


    <!-- http://www.parameter_estimation_ontology.org#sensor -->

    <owl:Class rdf:about="http://www.parameter_estimation_ontology.org#sensor">
        <rdfs:subClassOf rdf:resource="http://www.parameter_estimation_ontology.org#variable"/>
        <obo:IAO_0000115 xml:lang="en">A variable that corresponds to some experimentally measured data.</obo:IAO_0000115>
        <obo:IAO_0000117 xml:lang="en">PERSON: Alexander Klawonn</obo:IAO_0000117>
        <rdfs:label xml:lang="en">sensor</rdfs:label>
    </owl:Class>
    


    <!-- http://www.parameter_estimation_ontology.org#single_experiment_data_set -->

    <owl:Class rdf:about="http://www.parameter_estimation_ontology.org#single_experiment_data_set">
        <rdfs:subClassOf rdf:resource="http://purl.obolibrary.org/obo/IAO_0000100"/>
        <obo:IAO_0000115 xml:lang="en">A data set that is an aggregate of data recordings all of which have in common that they have been measured in a single experiment.</obo:IAO_0000115>
        <obo:IAO_0000117 xml:lang="en">PERSON: Alexander Klawonn</obo:IAO_0000117>
        <rdfs:label xml:lang="en">single experiment data set</rdfs:label>
    </owl:Class>
    


    <!-- http://www.parameter_estimation_ontology.org#truncated_normal_density_function -->

    <owl:Class rdf:about="http://www.parameter_estimation_ontology.org#truncated_normal_density_function">
        <rdfs:subClassOf rdf:resource="http://www.parameter_estimation_ontology.org#probability_density_function"/>
        <obo:IAO_0000115 xml:lang="en">A probability density function that is based on a normal distribution which has a primary variable with a bounded domain.</obo:IAO_0000115>
        <obo:IAO_0000117 xml:lang="en">PERSON: Alexander Klawonn</obo:IAO_0000117>
        <rdfs:label xml:lang="en">truncated normal density function</rdfs:label>
    </owl:Class>
    


    <!-- http://www.parameter_estimation_ontology.org#uniform_density_function -->

    <owl:Class rdf:about="http://www.parameter_estimation_ontology.org#uniform_density_function">
        <rdfs:subClassOf rdf:resource="http://www.parameter_estimation_ontology.org#probability_density_function"/>
        <obo:IAO_0000115 xml:lang="en">A probability density function that is based on a uniform distribution.</obo:IAO_0000115>
        <obo:IAO_0000117 xml:lang="en">PERSON: Alexander Klawonn</obo:IAO_0000117>
        <rdfs:label xml:lang="en">uniform density function</rdfs:label>
    </owl:Class>
    


    <!-- http://www.parameter_estimation_ontology.org#uninformative_density_function -->

    <owl:Class rdf:about="http://www.parameter_estimation_ontology.org#uninformative_density_function">
        <rdfs:subClassOf rdf:resource="http://www.parameter_estimation_ontology.org#probability_density_function"/>
        <obo:IAO_0000115 xml:lang="en">A probability density function that is constant over the entire domain of its primary variable.</obo:IAO_0000115>
        <obo:IAO_0000117 xml:lang="en">PERSON: Alexander Klawonn</obo:IAO_0000117>
        <rdfs:label xml:lang="en">uninformative density function</rdfs:label>
    </owl:Class>
    


    <!-- http://www.parameter_estimation_ontology.org#variable -->

    <owl:Class rdf:about="http://www.parameter_estimation_ontology.org#variable">
        <rdfs:subClassOf rdf:resource="http://purl.obolibrary.org/obo/IAO_0000029"/>
        <obo:IAO_0000115 xml:lang="en">A numeral that does not specify the number(s) it represents by their value (like constants do) but by stating numeric domain(s) it is chosen from.</obo:IAO_0000115>
        <obo:IAO_0000117 xml:lang="en">PERSON: Alexander Klawonn</obo:IAO_0000117>
        <rdfs:label xml:lang="en">variable</rdfs:label>
    </owl:Class>
    


    <!-- 
    ///////////////////////////////////////////////////////////////////////////////////////
    //
    // Individuals
    //
    ///////////////////////////////////////////////////////////////////////////////////////
     -->

    


    <!-- http://www.parameter_estimation_ontology.org#one -->

    <owl:NamedIndividual rdf:about="http://www.parameter_estimation_ontology.org#one">
        <rdf:type rdf:resource="http://www.parameter_estimation_ontology.org#constant"/>
    </owl:NamedIndividual>
    


    <!-- http://www.parameter_estimation_ontology.org#zero -->

    <owl:NamedIndividual rdf:about="http://www.parameter_estimation_ontology.org#zero">
        <rdf:type rdf:resource="http://www.parameter_estimation_ontology.org#constant"/>
    </owl:NamedIndividual>
</rdf:RDF>



<!-- Generated by the OWL API (version 4.5.9.2019-02-01T07:24:44Z) https://github.com/owlcs/owlapi -->

